theories/SubstExec.v
@@ -1,0 +1,71 @@
+(**
+
+This file contains a computable definition for [subst]. 
+
+Author: Arthur Charguéraud.
+License: MIT.
+
+*)
+
+Set Implicit Arguments.
+From Sep Require Import Semantics.
+Open Scope string_scope.
+
+(** [subst_exec] is like [subst] except that it computes with [simpl]. *)
+
+Fixpoint subst_exec (y:var) (w:val) (t:trm) : trm :=
+  let aux t := 
+    subst_exec y w t in
+  let bind_no_capture z t t' := 
+    match z with
+    | bind_anon => t'
+    | bind_var x => if var_eq x y then t else t'
+    end in
+  let aux_no_capture z t := 
+    bind_no_capture z t (aux t) in
+  let aux_no_captures xs t := 
+    if mem_exec var_eq y xs then t else aux t in
+  match t with
+  | trm_val v => trm_val v
+  | trm_var x => if var_eq x y then trm_val w else t
+  | trm_fixs f xs t1 => trm_fixs f xs (bind_no_capture f t1 (aux_no_captures xs t1))
+  | trm_constr id ts => trm_constr id (List.map aux ts)
+  | trm_if t0 t1 t2 => trm_if (aux t0) (aux t1) (aux t2)
+  | trm_let z t1 t2 => trm_let z (aux t1) (aux_no_capture z t2)
+  | trm_apps t0 ts => trm_apps (aux t0) (List.map aux ts)
+  | trm_while t1 t2 => trm_while (aux t1) (aux t2)
+  | trm_for x t1 t2 t3 => trm_for x (aux t1) (aux t2) (aux_no_capture x t3)
+  | trm_match t0 pts => trm_match (aux t0) (List.map (fun '(pi,ti) =>
+       (pi, aux_no_captures (patvars pi) ti)) pts)
+  | trm_fail => trm_fail
+  end.
+
+(** Proof of equivalence between [subst_exec] and [subst].
+    First, a few auxiliary lemmas. Then, then induction. *)
+
+Lemma eq_exec_var_eq : eq_exec var_eq.
+Proof using. intros x y. rewrite~ var_eq_spec. Qed.
+
+Lemma if_var_eq_spec : forall x y A (X Y:A),
+  (if var_eq x y then X else Y) = (If x = y then X else Y).
+Proof using. intros. rewrite var_eq_spec, if_classicT_eq_if_isTrue. auto. Qed.
+
+Lemma mem_exec_var_eq_eq : forall y xs,
+  mem_exec var_eq y xs = isTrue (mem y xs).
+Proof using. intros. applys mem_exec_eq. applys eq_exec_var_eq. Qed.
+
+Lemma subst_exec_eq_subst :
+  subst_exec = subst.
+Proof using.
+  applys fun_ext_3. intros y w t. induction t using trm_induct; simpl; fequals.
+  { rewrite~ if_var_eq_spec. }
+  { rewrite mem_exec_var_eq_eq. destruct b; [|try rewrite if_var_eq_spec];
+    repeat case_if; tryfalse; auto. } 
+  { rewrite List_map_eq. applys* map_congr. }
+  { destruct b; [|try rewrite if_var_eq_spec];
+    repeat case_if; tryfalse; auto. }
+  { rewrite List_map_eq. applys~ map_congr. }
+  { rewrite if_var_eq_spec. repeat case_if; auto. }
+  { rewrite List_map_eq. applys map_congr. intros (pi,ti) Mi. fequals.
+    rewrite mem_exec_var_eq_eq. rewrite if_classicT_eq_if_isTrue. case_if*. }
+Qed.
